

Student: Cole Lamers
Date: 09/26/19

Instructor: Viktoriya Shcherban
Course: Calc 1 11:30 AM / Internet
 (81749&81750) Shcherban

Assignment: 4.7 Antiderivatives (Set 1)

Find the antiderivative for each function when C equals 0. Do as many as you can mentally. Check your answers by differentiation.

a. $21x^{20}$ b. x^7 c. $x^2 + 2x - 48$

A derivative of the form $f(x) = x^n$ has a family of antiderivatives of the form $F(x) = \frac{1}{n+1}x^{n+1} + C$, where $n \neq -1$. Recall also the constant multiple rule, which states that $kf(x)$ has a general antiderivative of the form $kF(x) + C$, where k is a constant and $F(x)$ is the antiderivative of $f(x)$.

a. Let $f(x) = x^{20}$ and $k = 21$. For $f(x) = x^{20}$, identify the value of n to be used in the antiderivative formula.

$$n = 20$$

Substitute the value of n into the formula $F(x) = \frac{1}{n+1}x^{n+1} + C$ to find the antiderivative of $f(x) = x^{20}$ when $C = 0$.

$$f(x) = x^{20}$$

$$F(x) = \frac{1}{20+1}x^{20+1} \quad \text{Substitute and apply the constant multiple rule.}$$

$$= \frac{1}{21}x^{21} \quad \text{Simplify.}$$

b. For $f(x) = x^7$, identify the value of n to be used in the antiderivative formula.

$$n = 7$$

Substitute the value of n into the formula to find the antiderivative of $f(x) = x^7$ when $C = 0$.

$$f(x) = x^7$$

$$F(x) = \frac{1}{7+1}x^{7+1} \quad \text{Substitute.}$$

$$= \frac{1}{8}x^8 \quad \text{Simplify.}$$

c. Let $f(x) = g(x) + 2h(x) - 48p(x)$, where $g(x) = x^2$, $h(x) = x$, and $p(x) = x^0$. Then $F(x) = G(x) + 2H(x) - 48P(x) + C$ by a combination of the Sum or Difference Rule and the Constant Multiple Rule. Compute the antiderivative of each term individually. First, find $G(x)$ when $C = 0$. Note that $n = 2$ for the purposes of the antiderivative formula.

$$g(x) = x^2$$

$$G(x) = \frac{1}{2+1}x^{2+1} \quad \text{Substitute.}$$

$$= \frac{1}{3}x^3 \quad \text{Simplify.}$$

Now, find $H(x)$ when $C = 0$. Note that $n = 1$ for the purposes of the antiderivative formula.

$$h(x) = x$$

$$H(x) = \frac{1}{1+1}x^{1+1} \quad \text{Substitute.}$$

$$= \frac{1}{2}x^2 \quad \text{Simplify.}$$

Finally, find $P(x)$ when $C = 0$. Note that $n = 0$ for the purposes of the antiderivative formula.

$$p(x) = x^0$$

$$P(x) = \frac{1}{0+1}x^{0+1} \quad \text{Substitute.}$$

$$= x \quad \text{Simplify.}$$

To find $F(x)$ when $C = 0$, substitute the expressions found for $G(x)$, $H(x)$ and $P(x)$ into the equation $G(x) + 2H(x) - 48P(x)$ and simplify.

$$F(x) = G(x) + 2H(x) - 48P(x)$$

$$= \left(\frac{1}{3}x^3\right) + 2\left(\frac{1}{2}x^2\right) - 48(x) \quad \text{Substitute and apply the Constant Multiple Rule.}$$

$$= \frac{1}{3}x^3 + x^2 - 48x \quad \text{Simplify.}$$

Student: Cole Lamers
Date: 09/26/19

Instructor: Viktoriya Shcherban
Course: Calc 1 11:30 AM / Internet
(81749&81750) Shcherban

Assignment: 4.7 Antiderivatives (Set 1)

Find the indefinite integral $\int (8x + 3)dx$.

The Constant Multiple Rule, an antiderivative linearity rule, states that the general antiderivative for $k f(x)$ is $k F(x) + C$.

The Sum Rule, another antiderivative linearity rule, states that the general antiderivative for $[f(x) + g(x)]$ is $F(x) + G(x) + C$.

Alternative representations of these rules are

$$\int k f(x)dx = k \int f(x)dx = k F(x) + C$$

$$\text{and } \int (f(x) + g(x))dx = \int f(x)dx + \int g(x)dx = F(x) + G(x) + C.$$

Apply these same rules to the expression $\int (8x + 3)dx$.

First, apply the Sum Rule.

$$\int (8x + 3)dx = \int (8x)dx + \int 3 dx$$

Then apply the Constant Multiple Rule.

$$\int 8x dx = 8 \int x dx \text{ and } \int 3 dx = 3 \int dx$$

$$\int (8x + 3)dx = 8 \int x dx + 3 \int dx = 4x^2 + 3x + C$$

Student: Cole Lamers
Date: 09/26/19

Instructor: Viktoriya Shcherban
Course: Calc 1 11:30 AM / Internet
 (81749&81750) Shcherban

Assignment: 4.7 Antiderivatives (Set 1)

Find the most general antiderivative or indefinite integral. Check your answer by differentiation.

$$\int \left(3t^2 + \frac{t}{8} \right) dt$$

The sum rule for antiderivatives states that a sum of functions may be antidifferentiated term by term as given by the following formula.

$$\int [f(x) + g(x)] dx = \int f(x) dx + \int g(x) dx$$

Begin by writing the expression according to the sum rule.

$$\int \left(3t^2 + \frac{t}{8} \right) dt = \int 3t^2 dt + \int \frac{t}{8} dt$$

The constant multiple rule states that a constant multiple k may be moved through the integral sign as given by the following formula.

$$\int k f(x) dx = k \int f(x) dx$$

To antidifferentiate $\int 3t^2 dt$, first use the constant multiple rule to rewrite the expression.

$$\int 3t^2 dt = 3 \int t^2 dt$$

Now to antidifferentiate $3 \int t^2 dt$, use the formula $\int x^n dx = \frac{x^{n+1}}{n+1} + C$ and multiply by the constant 3.

$$3 \int t^2 dt = 3 \cdot \frac{t^3}{3} + C = t^3 + C$$

$$\text{Thus, } \int 3t^2 dt = t^3 + C.$$

Next use the constant multiple rule to rewrite $\int \frac{t}{8} dt$.

$$\int \frac{t}{8} dt = \frac{1}{8} \int t dt$$

Now to antidifferentiate $\frac{1}{8} \int t dt$, use the formula $\int x^n dx = \frac{x^{n+1}}{n+1} + C$ and multiply by the constant $\frac{1}{8}$.

$$\frac{1}{8} \int t dt = \frac{1}{8} \cdot \frac{t^2}{2} + C = \frac{t^2}{16} + C$$

$$\text{Thus, } \int \frac{t}{8} dt = \frac{t^2}{16} + C.$$

Now combine the separate terms to find the antiderivative of the original expression. For notational convenience, use only one constant of integration.

$$\begin{aligned}\int \left(3t^2 + \frac{t}{8} \right) dt &= \int 3t^2 dt + \int \frac{t}{8} dt \\ &= t^3 + \frac{t^2}{16} + C\end{aligned}$$

Check your answer by differentiation.

$$\frac{d}{dt} \left(t^3 + \frac{t^2}{16} + C \right) = 3t^2 + \frac{t}{8}$$

$$\text{Thus, } \int \left(3t^2 + \frac{t}{8} \right) dt = t^3 + \frac{t^2}{16} + C.$$

Student: Cole Lamers**Date:** 09/26/19**Instructor:** Viktoriya Shcherban**Course:** Calc 1 11:30 AM / Internet
(81749&81750) Shcherban**Assignment:** 4.7 Antiderivatives (Set 1)

Find the function $y(x)$ satisfying $\frac{dy}{dx} = 4x - 5$ and $y(3) = 0$.

First, find $y(x) = \int (4x - 5)dx$.

$$y(x) = \int (4x - 5)dx = 4 \int x \, dx - 5 \int dx$$

$$4 \int x \, dx = 2x^2 + C_1 \text{ and } 5 \int dx = 5x + C_2$$

$$\text{Letting } C = C_1 + C_2, \int (4x - 5)dx = 2x^2 - 5x + C.$$

$$\text{Thus, } y(x) = 2x^2 - 5x + C.$$

Since $y(3) = 0$, substitute 3 for x and 0 for $y(x)$.

$$2(3)^2 - 5(3) + C = 0$$

$$\text{Solving } 2(3)^2 - 5(3) + C = 0 \text{ for } C, C = -3.$$

Thus, the function $y(x)$ satisfying $\frac{dy}{dx} = 4x - 5$ and $y(3) = 0$ is $y(x) = 2x^2 - 5x - 3$.

Student: Cole Lamers**Date:** 09/26/19**Instructor:** Viktoriya Shcherban**Course:** Calc 1 11:30 AM / Internet
(81749&81750) Shcherban**Assignment:** 4.7 Antiderivatives (Set 1)

Find the function $s(t)$ satisfying $\frac{ds}{dt} = 5 - 3 \cos t$ and $s(0) = 4$.

$$\frac{ds}{dt} = 5 - 3 \cos t \text{ is equivalent to } s = \int (5 - 3 \cos t) dt.$$

Apply the Sum/Difference and Constant Multiple Rules.

$$\begin{aligned} s &= \int (5 - 3 \cos t) dt = \int 5 dt - \int 3 \cos t dt \\ &= 5 \int dt - 3 \int \cos t dt \\ &= 5t - 3 \sin t + C \end{aligned}$$

$$\text{Since } s(0) = 4, 5(0) - 3 \sin 0 + C = 4.$$

$$\text{Solving } 5(0) - 3 \sin 0 + C = 4 \text{ for } C, C = 4.$$

Thus, the function satisfying $\frac{ds}{dt} = 5 - 3 \cos t$ and $s(0) = 4$ is $s(t) = 5t - 3 \sin t + 4$.

Student: Cole Lamers**Date:** 09/26/19**Instructor:** Viktoriya Shcherban**Course:** Calc 1 11:30 AM / Internet
(81749&81750) Shcherban**Assignment:** 4.7 Antiderivatives (Set 1)

Find the function $y(x)$ satisfying $\frac{d^2y}{dx^2} = 4 - 12x$, $y'(0) = 5$, and $y(0) = 7$.

First, find $\frac{dy}{dx}$, the antiderivative of $\frac{d^2y}{dx^2} = 4 - 12x$.

$$\frac{dy}{dx} = \int (4 - 12x)dx = 4x - 6x^2 + C_1$$

The constant C_1 in $\frac{dy}{dx} = y' = 4x - 6x^2 + C_1$ can be evaluated by applying the initial value condition $y'(0) = 5$.

$$C_1 = 5$$

$$\text{So } \frac{dy}{dx} = y' = 4x - 6x^2 + 5.$$

$$y(x) = \int y' dx = \int (4x - 6x^2 + 5) dx = 2x^2 - 2x^3 + 5x + C_2$$

The constant C_2 in $y = 2x^2 - 2x^3 + 5x + C_2$ can be evaluated by applying the initial value condition $y(0) = 7$.

$$C_2 = 7$$

So, the function satisfying $\frac{d^2y}{dx^2} = 4 - 12x$, $y'(0) = 5$, and $y(0) = 7$ is $y(x) = 2x^2 - 2x^3 + 5x + 7$.